\documentclass[10pt]{article}
\usepackage[landscape, a4paper]{geometry}
\usepackage{JohnMath}
\usepackage{mathtools}

% The following sets text in Times, but keeps maths and tt in Computer Modern.
\renewcommand{\rmdefault}{ptm}

\usepackage[svgnames]{xcolor}

% CODE LISTINGS
\usepackage{listings}
\lstset{
  language=C,
  columns=[l]fullflexible,
  mathescape=true,
  basicstyle=\ttfamily\color{Black},
  showstringspaces=false,
  commentstyle=\color{DarkGreen}, 
  numbers=none, 
  escapechar=£,
  escapebegin={\normalsize\rmfamily\color{Black}}
}

% SPECIFICATIONS
\newcommand{\ml}[2][t]{\mbox{\mdseries\begin{tabular}[#1]{@{}L@{}}#2\end{tabular}}}
\newcommand{\ass}[1]{\ensuremath{{\color{blue}\left\{\ml[c]{#1}\right\}}}}
\newcommand{\seqspec}[3]{\ass{#1}\,{\mbox{{\tt #2}}}\,\ass{#3}}
\newcommand{\Seqspec}[3]{\multicolumn{2}{l}{$\ass{#1}$ {#2} $\ass{#3}$}}
\newcommand{\comm}[1]{\vspace{-2pt}%
    \begin{list}{/$*$}{%
        \topsep=5pt%
        \leftmargin=3cm%
      }\item #1 \hfill$*$/\end{list}%
}

\renewcommand{\arraystretch}{1.2}

\renewcommand{\true}{\mathsf{tt}}
\renewcommand{\emp}{\emph{emp}}

%\renewcommand{\boxed}[2][]{{\textbf{[}}#2{\textbf{]}}_{#1}}

\newcommand{\rsem}[1]{{(\![}{#1}{]\!)}}
%\newcommand{\iterstar}[2][]{\text{\LARGE $*$}^{#1}_{#2}}

\newcommand{\defined}{\mathop{\text{def}}}

\newcommand{\SET}[2]{\left\{\begin{array}{@{}l|l@{}} #1 & #2 \end{array}\right\}}

\newenvironment{mapping}{\left\{ \begin{array}{@{}r@{\,↦\,}l@{}}}{\end{array}\right\}}

%\newcommand{\block}[1]{\smash{\overbracket[0.5pt][2pt]{\underscore\,\ldots\,\underscore}^{#1}}}

% \newcommand{\ret}{\texttt{ret}}

% \newcommand{\malloc}{{\tt malloc}}
% \newcommand{\sbrk}{{\tt sbrk}}
% \newcommand{\free}{{\tt free}}
% \newcommand{\ls}[2][]{#1 \twoheadrightarrow #2}
% \newcommand{\arena}{\mathop{\emph{arena}}}
% \newcommand{\anArena}{\emph{anArena}}
% \newcommand{\token}{\mathop{\emph{token}}}
% \newcommand{\arenatoken}{\mathop{\emph{arenatoken}}}
% \newcommand{\block}{\mathop{\emph{block}}}
% \newcommand{\ublock}{\mathop{\emph{ublock}}}
% \newcommand{\ablock}{\mathop{\emph{ablock}}}
% \newcommand{\sblock}{\mathop{\emph{sblock}}}
% \newcommand{\A}[2][]{#1 \mathbin{\smash{\underset{\raisebox{3.5pt}{\smash{\sf\scriptsize a}}}{\rightarrow}}} #2}
% \newcommand{\U}[2][]{#1 \mathbin{\smash{\underset{\raisebox{3.5pt}{\smash{\sf\scriptsize u}}}{\rightarrow}}} #2}
% \newcommand{\B}[2][]{#1 {\rightarrow} #2}
% \newcommand{\E}[2]{#2 \mathbin{\raisebox{2pt}{$\curvearrowleft$}} #1}
% \newcommand{\s}{{\tt s}}
% \renewcommand{\t}{{\tt t}}
% \newcommand{\temp}{{\tt temp}}
% \newcommand{\p}{{\tt p}}
% \newcommand{\q}{{\tt q}}
% \renewcommand{\v}{{\tt v}}
% \newcommand{\brk}{\mathop{\emph{brk}}}
% \newcommand{\brka}{\mathop{\emph{brka}}}
% \newcommand{\n}{{}\\{} \hfill }
% \newcommand{\nw}{{\tt nw}}
% \newcommand{\ap}{{\tt ap}}
% \newcommand{\nbytes}{{\tt nbytes}}
% \newcommand{\WORD}{{\tt WORD}}
% \newcommand{\mathceil}[1]{\left\lceil#1\right\rceil}
% \newcommand{\ptoU}{\mathbin{↦_{\sf u}}}
% \newcommand{\ptoA}{\mathbin{↦_{\sf a}}}
% \newcommand{\ptoS}{\mathbin{↦_{\sf s}}}
% \newcommand{\uninit}{\mathop{\emph{uninit}}}
\newcommand{\arity}{\mathop{\mathit{arity}}}
\newcommand{\loc}[1]{\mathop{\mathit{loc}}(#1)}
\newcommand{\sha}[1]{\mathop{\mathit{sha}}(#1)}
\newcommand{\lift}[1]{\mathop{\mathit{lift}}(#1)}
\newcommand{\pullout}[1]{\underline{#1}}

\title{GSep}
\author{John Wickerson}
\date{}

\begin{document}

\maketitle

\newcommand{\ret}{\texttt{ret}}
\newcommand{\WR}{\mathop{\mathit{wr}}}
\newcommand{\RD}{\mathop{\mathit{rd}}}

\section{Separation Logic with Modules and Abstract Predicates}

%\subsection{Semantic model}
% \[
% \begin{array}{rclcl}
% X &∈& \mathbb{LV} \\
% x &∈& \mathbb{PV} \\
% % && \mathbb{V} &\eqdef& \mathbb{LV} ∪ \mathbb{PV} \\
% v &∈& {\sf Val} \\
% C &∈& {\sf Com} \\
% C &∈& {\sf ClosedCom} &\eqdef& \{C∈{\sf Com}\mid \mods(C) = ∅\} \\
% α &∈& \mathbb{A} \\
% \arity{} &:& & & \mathbb{A} → \mathbb{N} \\
% f &∈& \mathbb{F} \\
% \arity{} &:& & & \mathbb{F} → \mathbb{N} \\
% s &∈& {\sf Store} &\eqdef& \mathbb{PV} → {\sf Val} \\
% h &∈& {\sf Heap} &\eqdef& \mathbb{N} \rightharpoonup {\sf Val} \\
% %i &∈& {\sf LogEnv} &\eqdef& \mathbb{LV} → {\sf Val} \\
% %σ &∈& {\sf State} &\eqdef& {\sf Store} × {\sf Heap} × {\sf LogEnv} \\
% Π &∈& {\sf PredEnv} &\eqdef& (a:\mathbb{A}) → {\sf Val}^{\arity(a)} → {\sf Store} → {\sf Heap} → 2 \\
% Δ,P,Q &∈& {\sf Assn} \\
% ⊧ &:&  & & {\sf Assn} → {\sf PredEnv} → {\sf Store} → {\sf Heap} → 2 \\
% %\bold P, \bold Q &∈& {\sf ParaAssn} &\eqdef& {\sf Val}^* → {\sf Assn} \\
% F &∈& {\sf ProcImps} &\eqdef& (f:\mathbb{F}) → ({\sf Val}^{\arity(f)} → {\sf ClosedCom}) \\
% Γ &∈& {\sf ProcSpecs} &\eqdef& (f:\mathbb{F}) \rightharpoonup (({\sf Val}^{\arity(f)} → {\sf Assn}) × ({\sf Val}^{\arity(f)} → {\sf Assn})) \\
% \end{array}
% \]

Let $x$ range over the set $\mathbb{LV}$ of logical variables, and $X$ range over the set $\mathbb{PV}$ of program variables. Let $v$ range over a set ${\sf Val}$ of values. Let $C$ range over a language ${\sf Com}$ of commands. 
\[
C ::= C;C \mid \ang{C} \mid C+C \mid C^* \mid c \mid \texttt{let} (k_i = C_i)_{i∈n} \texttt{in} C \mid \texttt{call} k
\]
Let $k$ range over a set $\mathbb{K}$ of procedure identifiers. Let $K$ range over the set 
\[
{\sf ProcImps} \eqdef \mathbb{K} → {\sf Com}
\]
of procedure implementations that associate each procedure identifier with a closed command. We have a small-step operational semantics for commands. 
\begin{mathpar}
(C,σ) →_K (C',σ')   \and    (C,σ) →_K \emph{fault}
\end{mathpar}
Let $s$ range over the set ${\sf Store} \eqdef \mathbb{PV} → {\sf Val}$ of mappings from program variables to values. Let $h$ range over the set ${\sf Heap} \eqdef \mathbb{N} \rightharpoonup {\sf Val}$ of partial mappings from heap locations (natural numbers) to values. Let $α$ range over a set $\mathbb{A}$ of abstract predicate identifiers. Let $Π$ range over the set 
\[
{\sf PredEnv} \eqdef \mathbb{A} → \pow({\sf Store} × {\sf Heap})
\]
of predicate environments that associate each abstract predicate with a set of states that it satisfies. Let $P,Q$ range over a language ${\sf Assn}$ of assertions.
\[
P ::= P * P \mid α \mid \dots
\]
There exists a forcing relation $s,h ⊧_Π P$ that describes when a state $(s,h)$ satisfies an assertion $P$ which may refer to abstract predicates defined in $Π$.
\begin{mathpar}
s,h ⊧_Π P*Q \eqdef ∃h_0,h_1．h = h_0 \uplus h_1 ∧ s,h_0 ⊧_Π P ∧ s,h_1 ⊧_Π Q
\and
s,h ⊧_Π α \eqdef (s,h) ∈ Π(α)
\end{mathpar}
Let $Δ$ range over the set ${\sf PredDict} = \mathbb{A} \rightharpoonup {\sf Assn}$ of abstract predicate dictionaries that associate some abstract predicates with an assertion. We write $Π ⊧ Δ$ to mean 
\[
∀(α↦P) ∈ Δ．Π(α) = \{(s,h) \mid s,h ⊧_Π P\}.
\]
We write $Δ ⊧ P⇒Q$ to mean 
\[
∀Π⊧Δ．∀s,h．(s,h)⊧_Π P ⇒ (s,h)⊧_Π Q.
\]
Let $Γ$ range over the set 
\[
{\sf ProcSpecs} \eqdef \mathbb{K} \rightharpoonup ({\sf Assn} × {\sf Assn})
\]
of procedure specifications that associate some procedure identifiers with a pre- and postcondition.


\newcommand{\safe}{\mathop{\mathit{safe}}}

\begin{defn} $\safe(Q,K,Π)$ is the largest set such that if $(C,s,h) ∈ \safe(Q,K,Π)$ then:
\begin{itemize}
\item $∀h_o,h_1．h\uplus h_o = h_1 ⟹ ¬\ang{C,(s,h_1)}→_K\emph{fault}$
\item $C = \Skip ⟹ (s,h) ⊧_Π Q$
\item $∀C',s',h',h_o,h_1．h\uplus h_o = h_1 ∧ \ang{C,(s,h_1)}→_K\ang{C',(s',h'_1)} ⟹ ∃h'．h' \uplus h_o = h'_1 ∧ (C',s',h') ∈ \safe(Q,K,Π)$
\end{itemize}
\end{defn}

% \begin{defn}\label{defn:sep_spec_inner}
% \[
% \ml{
% Δ ⊧_K \{P\}\,C\,\{Q\}  \eqdef 
% \ml{
% ∀s,h,Π．\\
% \text{if } Π⊧Δ \text{ and } s,h ⊧_Π P \\
% \text{then } \ml{ ∀h_o,h_1．h\uplus h_o = h_1 ⟹ ¬\ang{C,s,h_1,K}\lightning \\
% \text{and } \ml{ ∀s',h',h_o,h_1．\\
% \text{if } h\uplus h_o = h_1 ∧ \ang{C,s,h_1,K}⇓(s',h'_1) \\ 
% \text{then } ∃h'．h' \uplus h_o = h'_1 ∧ s',h' ⊧_Π Q}
% }
% }
% }
% \]
% \end{defn}

\begin{defn}
\[
Π;K ⊧ \{P\}\,C\,\{Q\}  \eqdef  ∀(s,h) ⊧_Π P． (C,s,h) ∈ \safe(Q,K,Π) 
\]
\end{defn}

\begin{defn}
\[
\ml{
K ⊧_Π Γ ~\eqdef~ ∀\{P\}\,k\,\{Q\}∈Γ．Π;K ⊧ \{P\}\,K\,k\,\{Q\}
}
\]
\end{defn}

\begin{defn}\label{defn:sep_spec}
\[
Δ;Γ⊧\{P\}\,C\,\{Q\}  \eqdef  ∀Π ⊧ Δ． ∀K ⊧_Π Γ． Π;K ⊧  \{P\}\,C\,\{Q\}
\]
\end{defn}

% \subsection{Proof rules}

%All the normal ones, plus the hypothetical frame rule, below. I've adapted the rule to include a $C_{\rm init}$ command that initialises all the variables declared at the top level of the module.

% We have the following proof rule.

% \[
% \inferrule[HypFrame]{
% (Δ;Γ ⊦ \{P_i * R\}\,C_i\,\{Q_i * R\})_{i∈n} \\\\
% Δ;Γ⊦\{P\}\,C_{\rm init}\,\{P'*R\} \\\\
% Δ;Γ⊦\{Q'*R\}\,C_{\rm final}\,\{Q\} \\\\
% Δ; Γ,(\{P_i\}\,f_i\,\{Q_i\})_{i∈n} ⊦ \{P'\}\,C\,\{Q'\}}
% {Δ;Γ ⊦ \{P\}\,\texttt{module} (C_{\rm init};(f_i = C_i)_{i∈n};C_{\rm final}) \texttt{in} C\,\{Q\}}
% \]


\section{GSep}

\subsection{Extension to semantic model}

Define $X \otimes Y \eqdef \{(x,y)\mid x\perp y\}$. Let $π$ range over the set 
\[
{\sf GPredEnv} \eqdef \mathbb{A} → \pow({\sf Store} × ({\sf Heap} \otimes {\sf Heap}))
\]
of GSep predicate environments that associate each abstract predicate with a set of GSep states it satisfies. If $π∈{\sf GPredEnv}$ then $\loc{π}$ and $\sha{π}$ are elements of {\sf PredEnv} such that 
\begin{mathpar}
\loc{π}(α) = \{(s,h_L)\mid ∃h_S．(s,h_L,h_S) ∈ π(α)\}
\and
\sha{π}(α) = \{(s,h_S)\mid (s,∅,h_S) ∈ π(α)\}
\end{mathpar}
and if $Π ∈ {\sf PredEnv}$ then $\lift{Π}$ is an element of {\sf GPredEnv} such that
\[
\lift{Π}(α) = \{(s,h_L,h_S)\mid h_S\perp h_L ∧ (s,h_L) ∈ Π(α)\}.
\]
\begin{lemma}
 $π(α) ⊆ \lift{\loc{π}}(α)$ for all $α$
\end{lemma}
\begin{proof}
Fix arbitrary $α$, $s$, $h_L$ and $h_S$.
\begin{eqnarray*}
(s,h_L,h_S) ∈ \lift{\loc{π}}(α) &=& h_S \perp h_L ∧ (s,h_L) ∈ \loc{π}(α) \\
&=& h_S \perp h_L ∧ (∃h_S．(s,h_L,h_S) ∈ π(α)) \\
&⇐& (s,h_L,h_S) ∈ π(α)
\end{eqnarray*}
\end{proof}
\begin{lemma}
$\loc{\lift{Π}} = Π$
\end{lemma}
\begin{proof} Fix arbitrary $α$, $s$ and $h_L$.
\begin{eqnarray*}
(s,h_L) ∈ \loc{\lift{Π}}(α) &=& ∃h_S．(s,h_L,h_S) ∈ \lift{Π}(α) \\
&=& ∃h_S．h_S \perp h_L ∧ (s,h_L) ∈ Π(α) \\
&=& (s,h_L) ∈ Π(α)
\end{eqnarray*}
\end{proof}
Let $G$ range over the set {\sf Guar} of binary relations on ${\sf Heap}$. Let $p,q$ range over a language {\sf GAssn} of GSep assertions. 
\[
p ::= \boxed{P} \mid P \mid p*p \mid \underline{α} \mid \dots
\]
There exists a forcing relation $s,h_L,h_S ⊧_π p$ that describes when a GSep state $(s,(h_L,h_S))$ satisfies a GSep assertion $p$ which may refer to abstract predicates defined in $π$.
\begin{mathpar}
s,h_L,h_S ⊧_π P \eqdef s,h_L ⊧_{\loc{π}} P
\and
s,h_L,h_S ⊧_π \boxed{P} \eqdef s,h_S ⊧_{\sha{π}} P ∧ h_L=∅
\and
s,h_L,h_S ⊧_π p*q \eqdef ∃h'_L,h''_L．h_L = h'_L \uplus h''_L ∧ s,h'_L,h_S ⊧_π p ∧ s,h''_L,h_S ⊧_π q
\and
s,h_L,h_S ⊧_π \underline{α} \eqdef (s,h_L,h_S) ∈ π(α)
\end{mathpar}
Let $δ$ range over the set ${\sf GPredDict} = \mathbb{A} \rightharpoonup {\sf GAssn}$ of abstract predicate dictionaries that associate some abstract predicates with a GSep assertion. Note that every {\sf PredDict} is a {\sf GPredDict}. We write $π ⊧ δ$ to mean 
\[
∀(α↦p) ∈ δ．π(α) = \{(s,h_L,h_S) \mid s,h_L,h_S ⊧_π p\}.
\]
\begin{lemma}
$Π⊧Δ$ iff $\lift{Π} ⊧ Δ$.
\end{lemma}
\begin{proof}
\begin{eqnarray*}
\lift{Π} ⊧ Δ &=& ∀(α↦P) ∈ Δ．\lift{Π}(α) = \{(s,h_L,h_S)\mid s,h_L,h_S ⊧_{\lift{Π}} P\} \\
&=& ∀(α↦P) ∈ Δ．∀s,h_L,h_S．(h_S\perp h_L ∧ (s,h_L)∈Π(α)) ⇔ s,h_L,h_S ⊧_{\lift{Π}} P \\ 
&=& ∀(α↦P) ∈ Δ．∀s,h_L,h_S．(h_S\perp h_L ∧ (s,h_L)∈Π(α)) ⇔ s,h_L ⊧_{\loc{\lift{Π}}} P \\ 
&=& ∀(α↦P) ∈ Δ．∀s,h_L,h_S．(h_S\perp h_L ∧ (s,h_L)∈Π(α)) ⇔ s,h_L ⊧_Π P \\ 
&=& ∀(α↦P) ∈ Δ．∀s,h_L．(∃h_S．h_S\perp h_L ∧ (s,h_L)∈Π(α)) ⇔ s,h_L ⊧_Π P \\ 
&=& ∀(α↦P) ∈ Δ．∀s,h_L．(s,h_L)∈Π(α) ⇔ s,h_L ⊧_Π P \\ 
&=& Π ⊧ Δ 
\end{eqnarray*}
\end{proof}
\begin{lemma}
$π⊧Δ$ iff $\loc{π} ⊧ Δ$.
\end{lemma}
\begin{proof}
\begin{eqnarray*}
\loc{π} ⊧ Δ &=& ∀(α↦P) ∈ Δ．∀s,h_L．(s,h_L)∈\loc{π}(α) ⇔ s,h_L ⊧_{\loc{π}} P \\
&=& ∀(α↦P) ∈ Δ．∀s,h_L．(s,h_L)∈\loc{π}(α) ⇔ s,h_L ⊧_{\loc{π}} P \\
&=& ∀(α↦P) ∈ Δ．∀s,h_L．(∃h_S．(s,h_L,h_S) ∈ π(α)) ⇔ s,h_L ⊧_{\loc{π}} P \\
&=& ∀(α↦P) ∈ Δ．∀s,h_L,h_S．(s,h_L,h_S) ∈ π(α) ⇔ s,h_L ⊧_{\loc{π}} P \\
&=& ∀(α↦P) ∈ Δ．π(α) = \{(s,h_L,h_S)\mid s,h_L ⊧_{\loc{π}} P\} \\
&=& ∀(α↦P) ∈ Δ．π(α) = \{(s,h_L,h_S)\mid s,h_L,h_S ⊧_π P\}
\end{eqnarray*}
\end{proof}
We write $δ ⊧_{\sf G} p⇒q$ to mean 
\[
∀π⊧δ．∀s,h_L,h_S．(s,h_L,h_S)⊧_π p ⇒ (s,h_L,h_S)⊧_π q.
\]
\begin{lemma}
In the case where $p$ and $q$ are local assertions and $δ$ is a local predicate dictionary, we have:
\[
(Δ ⊧_{\sf G} P⇒Q) = (Δ ⊧ P⇒Q)
\]
\end{lemma}
\begin{proof}
\begin{eqnarray*}
Δ ⊧_{\sf G} P⇒Q &=& ∀π．π⊧Δ ⟹ ∀s,h_L,h_S．(s,h_L,h_S)⊧_π P ⇒ (s,h_L,h_S)⊧_π Q \\
&=& ∀π．\loc{π}⊧Δ．∀s,h_L,h_S．(s,h_L,h_S)⊧_π P ⇒ (s,h_L,h_S)⊧_π Q \\
&=& ∀π．\loc{π}⊧Δ．∀s,h_L,h_S．(s,h_L)⊧_{\loc{π}} P ⇒ (s,h_L)⊧_{\loc{π}} Q \\
&=& ∀Π．Π⊧Δ．∀s,h_L,h_S．(s,h_L)⊧_Π P ⇒ (s,h_L)⊧_Π Q \\
&=& Δ ⊧ P⇒Q
\end{eqnarray*}
\end{proof}
As a result of the above lemma, we can drop the {\sf G} subscript in the sequel. Let $γ$ range over the set
\[
{\sf GProcSpecs} \eqdef \mathbb{K} \rightharpoonup ({\sf GAssn} × {\sf GAssn} × {\sf Guar})
\]
of procedure specifications that associate some procedure identifiers with a pre- and postcondition in {\sf GAssn} plus a guarantee. The following function converts an {\sf Assn} into an {\sf GAssn} by underlining all of the abstract predicates (thus allowing their values to range over the shared state not just the local state).
\begin{mathpar}
\pullout{P*Q} \eqdef \pullout{P} * \pullout{Q}
\and
\pullout{α} \eqdef \pullout{α}
\and
\dots
\end{mathpar}
We can convert elements of {\sf ProcSpecs} to elements of {\sf GProcSpecs} like so:
\[
Γ[G] = \{ \{P\}k\{Q\}[G] \mid \{P\}k\{Q\} ∈ Γ\}
\]

% We extend our model as follows:
% \[
% \begin{array}{rclcl}
% %w &∈& {\sf World} &\eqdef& \{(σ_l,σ_s)\mid σ_l,σ_s ∈ {\sf State} ∧ σ_l \perp σ_s\} \\
% π &∈& {\sf GPredEnv} &\eqdef& (α:\mathbb{A}) → ({\sf Val}^{\arity(α)} → \pow({\sf World})) \\
% G &∈& {\sf Guar} &\eqdef& \pow({\sf World}×{\sf World}) \\
% δ,p,q &∈& {\sf GAssn} &\eqdef& {\sf GPredEnv} → \pow({\sf World}) \\
% γ &∈& {\sf GProcSpecs} &\eqdef& (f:\mathbb{F}) \rightharpoonup (\mathbb{PV}^{\arity(f)} → {\sf GAssn} × {\sf GAssn}) \\
% \end{array}
% \]

\begin{defn} $\safe(q,K,π,G)$ is the largest set such that if $(C,s,h_L,h_S) ∈ \safe(q,K,π,G)$ then:
\begin{itemize}
\item $∀h_o,h．h_L\uplus h_S\uplus h_o = h ⟹ ¬\ang{C,(s,h)}→_K\emph{fault}$
\item $C = \Skip ⟹ (s,h_L,h_S) ⊧_π q$
\item $∀C',s',h'_S,h'_L,h_o,h．h_L\uplus h_S\uplus h_o = h ∧ \ang{C,(s,h)}→_K\ang{C',(s',h')} ⟹ ∃h'_L, h'_S．h'_L \uplus h'_S \uplus h_o = h' ∧ (h_S,h'_S) ∈ G ∧ (C',s',h'_L,h'_S) ∈ \safe(q,K,π,G)$
\end{itemize}
\end{defn}

% \begin{defn}\label{defn:sep_spec_inner}
% \[
% \ml{
% Δ ⊧_K \{P\}\,C\,\{Q\}  \eqdef 
% \ml{
% ∀s,h,Π．\\
% \text{if } Π⊧Δ \text{ and } s,h ⊧_Π P \\
% \text{then } \ml{ ∀h_o,h_1．h\uplus h_o = h_1 ⟹ ¬\ang{C,s,h_1,K}\lightning \\
% \text{and } \ml{ ∀s',h',h_o,h_1．\\
% \text{if } h\uplus h_o = h_1 ∧ \ang{C,s,h_1,K}⇓(s',h'_1) \\ 
% \text{then } ∃h'．h' \uplus h_o = h'_1 ∧ s',h' ⊧_Π Q}
% }
% }
% }
% \]
% \end{defn}

\begin{defn}
\[
π;K ⊧ \{p\}\,C\,\{q\}[G]  \eqdef  ∀(s,h_L,h_S) ⊧_π p． (C,s,h_L,h_S) ∈ \safe(q,K,π,G) 
\]
\end{defn}

\begin{defn}
\[
\ml{
K ⊧_π γ ~\eqdef~ ∀\{p\}\,k\,\{q\}[G]∈γ．π;K ⊧ \{p\}\,K\,k\,\{q\}[G]
}
\]
\end{defn}

\begin{defn}\label{defn:sep_spec}
\[
δ;γ⊧\{p\}\,C\,\{q\}[G]  \eqdef  ∀π⊧δ．∀K ⊧_π γ．π;K ⊧ \{p\}\,C\,\{q\}[G]
\]
\end{defn}

% \begin{defn}
% \[
% \ml{
% δ;G ⊧_K \{p\}\,C\,\{q\}  \eqdef 
% \ml{
% ∀s,h_L,h_S,π．\\
% \text{if } π⊧δ \text{ and } s,h_L,h_S ⊧_π p \\
% \text{then } \ml{ ∀h_o,h．h_L\uplus h_S \uplus h_o = h ⟹ ¬\ang{C,s,h,K}\lightning \\
% \text{and } \ml{ ∀s',h',h_o,h．\\
% \text{if } h_L\uplus h_S\uplus h_o = h ∧ \ang{C,s,h,K}⇓(s',h') \\ 
% \text{then } ∃h'_L,h'_S．h'_L \uplus h'_S \uplus h_o = h' ∧ (h_S, h'_S) ∈ G ∧ s',h'_L,h'_S ⊧_Π q}
% }
% }
% }
% \]
% \end{defn}

% \begin{defn}
% \[
% \ml{
% K ⊧ (γ,δ,G) ~\eqdef~ ∀\{p\}\,k\,\{q\}∈γ．δ;G ⊧_K \{p\}\,K\,k\,\{q\}
% }
% \]
% \end{defn}

% \begin{defn}
% \[
% δ;γ;G ⊧ \{p\}\,C\,\{q\}  \eqdef  ∀K ⊧ (γ,δ,G)． δ ⊧_K  \{p\}\,C\,\{q\}
% \]
% \end{defn}


% \subsection{Additional proof rules}

% \noindent Weakening the environment:
% \[
% \inferrule*[right=Env-Weaken]
% {δ';γ';G' ⊦ \{p\}\,C\,\{q\} \\ δ ⇒ δ' \\ γ ⇒ γ' \\ G' ⊆ G}
% {δ;γ;G ⊦ \{p\}\,C\,\{q\}}
% \]

% \noindent Rule of consequence:
% \[
% \inferrule*[right=Conseq]
% {δ;γ;G ⊦ \{p\}\,C\,\{q\} \\ (δ ∧ p) ⇒ p' \\ (δ ∧ q') ⇒ q}
% {δ;γ;G ⊦ \{p\}\,C\,\{q\}}
% \]

% \noindent Frame rule
% \[
% \inferrule*[right=Frame]
% {δ;γ;G ⊦ \{p\}\,C\,\{q\} \\ r \text{stable under} G}
% {δ;γ;G ⊦ \{p*r\}\,C\,\{q*r\}}
% \]

% \noindent Region update
% \[
% \inferrule*[right=RegUpdate]
% {δ;γ ⊦ \{P*P'\}\,C\,\{∃x．Q*Q'\} \\ (P \rightsquigarrow ∃x．Q) ⊆ G \\ P, Q  \text{precise}}
% {δ;γ;G ⊦ \{\boxed{R*P}*P'\}\,C\,\{∃x．\boxed{R*Q}*Q'\}}
% \]



% \noindent Converting between sequential and GSep specifications
% \begin{mathpar}
% \inferrule*[right=Basic]{Δ;Γ⊦\{P\}\,C\,\{Q\}}{G;Δ;Γ ⊦ \{P\}\,C\,\{Q\}}
% \and
% \inferrule*[right=Erase]{G;Δ;Γ⊦\{P\}\,C\,\{Q\}}{Δ;Γ ⊦ \{P\}\,C\,\{Q\}}
% \end{mathpar}

\section{Proof rules}


\begin{mathpar}
\inferrule[Underline]{
}{
Δ ⊧ \underline{P} ⇒ P
}
\and
\inferrule[G-Erase]{
Δ;Γ[G] ⊦ \{P*\boxed{P'}\}\,C\,\{Q*\boxed{Q'}\}[G]
}{
Δ;Γ ⊦ \{P*P'\}\,C\,\{Q*Q'\}
}
\and
\inferrule[G-Basic]{
Δ;Γ ⊦ \{P\}\,C\,\{Q\}
}{
Δ;Γ[G] ⊦ \{P\}\,C\,\{Q\}[G]
}
\and
\inferrule[Proc-Conseq]{
δ ⊧ p' ⇒ p \\ δ ⊧ q ⇒ q' \\ G ⊆ G' \\\\ δ;γ\uplus\{p'\}k\{q'\}[G'] ⊦ \{p_0\}\,C\,\{q_0\}[G_0]
}{
δ;γ\uplus\{p\}k\{q\}[G] ⊦ \{p_0\}\,C\,\{q_0\}[G_0]
}
\and
\inferrule[Conseq]{
δ ⊧ p ⇒ p' \\ δ ⊧ q' ⇒ q \\ G' ⊆ G \\\\ δ;γ ⊦ \{p'\}\,C\,\{q'\}[G']
}{
δ;γ ⊦ \{p\}\,C\,\{q\}[G]
}
\and
\inferrule[G-PredE]{
δ\uplus δ';Γ ⊦ \{p\}\,C\,\{q\}[G] \\\\ ∀α∈\dom(δ')．α∉δ,Γ,p,q 
}{
δ;Γ ⊦ \{p\}\,C\,\{q\}[G]
}
\and
\inferrule[G-PredI]{
δ;Γ ⊦ \{p\}\,C\,\{q\}[G]
}{
δ\uplus δ';Γ ⊦ \{p\}\,C\,\{q\}[G]
}
\and
\inferrule[G-HypFrame] {
δ;Γ \uplus (\{p_i\}k_i\{q_i\}[G_i])_{i∈n} ⊦ \{p\}\,C\,\{q\}[G]
}{
δ;Γ \uplus (\{p_i*r\}k_i\{q_i*r\}[G_i])_{i∈n} ⊦ \{p*r\}\,C\,\{q*r\}[G]
}
\and
\inferrule[G-Let] {
(δ;γ ⊦ \{p_i\}\,C_i\,\{q_i\}[G])_{i∈n}
\\\\
δ;γ \uplus (\{p_i\}k_i\{q_i\}[G])_{i∈n} ⊦ \{p\}\,C\,\{q\}[G]
}{
δ;γ ⊦ \{p\}\,\texttt{let} (f_i = C_i)_{i∈n} \texttt{in} C\,\{q\}[G]
}
\end{mathpar}

\noindent The following rule....

\[
\inferrule[G-DerivModule] {
(Δ\uplus δ;Γ ⊦ \{ \pullout{P_i} * \boxed{R}\}\,C_i\,\{\pullout{Q_i} * \boxed{R}\}[G])_{i∈n}
\\\\
Δ;Γ \uplus (\{P_i\}k_i\{Q_i\})_{i∈n} ⊦ \{P\}\,C\,\{Q\}
}{
Δ;Γ ⊦ \{P*R\}\,\texttt{let} (f_i = C_i)_{i∈n} \texttt{in} C\,\{Q*R\} 
}
\]

\noindent ... can be derived like so:

\[
\inferrule*[Right=G-Let] {
(Δ \uplus δ;Γ ⊦ \{ \pullout{P_i} * \boxed{R}\}\,C_i\,\{\pullout{Q_i} * \boxed{R}\}[G])_{i∈n} 
\\
\inferrule*[Right=HypFrame] { 
\inferrule*[Right=Proc-Conseq] {
\dom(δ) = {\textstyle \bigcup_{i∈n} ap(P_i ∨ Q_i)}
\\
\inferrule*[Right=G-PredI] {
\inferrule*[Right=G-Basic] {
Δ;Γ \uplus (\{P_i\}k_i\{Q_i\})_{i∈n} ⊦ \{P\}\,C\,\{Q\}
}{
Δ;Γ[G] \uplus (\{P_i\}k_i\{Q_i\}[G])_{i∈n} ⊦ \{P\}\,C\,\{Q\}[G]
}
}{
Δ\uplus δ;Γ[G] \uplus (\{P_i\}k_i\{Q_i\}[G])_{i∈n} ⊦ \{P\}\,C\,\{Q\}[G]
}
}{
Δ\uplus δ;Γ[G] \uplus (\{\pullout{P_i}\}k_i\{\pullout{Q_i}\}[G])_{i∈n} ⊦ \{P\}\,C\,\{Q\}[G]
}
}{
Δ\uplus δ;Γ[G] \uplus (\{\pullout{P_i}*\boxed{R}\}k_i\{\pullout{Q_i}*\boxed{R}\}[G])_{i∈n} ⊦ \{P*\boxed{R}\}\,C\,\{Q*\boxed{R}\}[G]
}
}{
\inferrule*[Right=G-PredE] {
Δ\uplus δ;Γ[G] ⊦ \{P*\boxed{R}\}\,\texttt{let} (f_i = C_i)_{i∈n} \texttt{in} C\,\{Q*\boxed{R}\}[G]
}{
\inferrule*[Right=G-Erase] {
Δ;Γ[G] ⊦ \{P*\boxed{R}\}\,\texttt{let} (f_i = C_i)_{i∈n} \texttt{in} C\,\{Q*\boxed{R}\}[G]
}{
Δ;Γ ⊦ \{P*R\}\,\texttt{let} (f_i = C_i)_{i∈n} \texttt{in} C\,\{Q*R\} 
}
}
}
\]

\section{Soundness?}


\subsection{Underline}

Fix arbitrary $π⊧Δ$. Show $∀P．∀s,h_L,h_S．(s,h_L,h_S ⊧_π P) ⇐ (s,h_L,h_S ⊧_π \underline{P})$ by induction on $P$.

Case $P = α$. Suppose $α∈\dom(Δ)$. Hence $(s,h_L,h_S) ∈ π(α) ⇔ s,h_L,h_S ⊧_π Δ(α)$.
\begin{eqnarray*}
s,h_L,h_S ⊧_π α &=& h_S \perp h_L ∧ s,h_L ⊧_{\loc{π}} α \\
&=& h_S \perp h_L ∧ (s,h_L) ∈ {\loc{π}}(α) \\
&=& h_S \perp h_L ∧ (∃h_S．(s,h_L,h_S) ∈ π(α)) \\
&=& h_S \perp h_L ∧ (∃h_S．s,h_L,h_S ⊧_π Δ(α)) \\
&=& h_S \perp h_L ∧ (∃h_S．s,h_L ⊧_{\loc{π}} Δ(α)) \\
&=& h_S \perp h_L ∧ s,h_L ⊧_{\loc{π}} Δ(α) \\
&=& s,h_L,h_S ⊧_π Δ(α) \\
&=& (s,h_L,h_S) ∈ π(α) \\
&=& s,h_L,h_S ⊧_π \underline{α}
\end{eqnarray*}

Case $P = P' * P''$.
\begin{eqnarray*}
s,h_L,h_S ⊧_π P'*P'' &=& ∃h'_L,h''_L．h_L = h'_L \uplus h''_L ∧ s,h'_L,h_S ⊧_π P' ∧ s,h''_L,h_S ⊧_π P'' \\
&⇐& ∃h'_L,h''_L．h_L = h'_L \uplus h''_L ∧ s,h'_L,h_S ⊧_π \underline{P'} ∧ s,h''_L,h_S ⊧_π \underline{P''} \\
&=& s,h_L,h_S ⊧_π \underline{P'}*\underline{P''} \\
&=& s,h_L,h_S ⊧_π \underline{P'*P''}
\end{eqnarray*}




\begin{lemma}[G-Erase 1]
If $s,h_L,h_S ⊧_Π \underline P$ then $s,h_L ⊧_Π P$.
\end{lemma}

\begin{lemma}[G-Erase 2]
If $(C,s,h_L) ∈ \safe(Q,K,Π)$ then $(C,s,h_L,h_S) ∈ \safe(\underline Q,K,Π,G)$.
\end{lemma}


\subsection{G-Erase}

Suppose $Δ⊧\{P\}C\{Q\}$. Show $G;Δ⊧\{\underline P\}C\{Q\}$. Fix arbitrary $K$. No procedure environment, so $K$ not used. Fix arbitrary $π$. Assume $π⊧Δ$. Then $π = Π$ for some $Π$. Assume $s,h_L,h_S ⊧_Π \underline P$. Then $s,h_L ⊧_Π P$ by lemma. So $(C,s,h_L) ∈ \safe(Q,K,Π)$ by assumption. Then we need $(C,s,h_L,h_S) ∈ \safe(\underline Q,K,Π,G)$ too.

\end{document}